src/lib/poly/gemm/Kuiper.Poly.GEMM.BlockTiling1D.fst
@@ -29,6 +29,12 @@ open Kuiper.ArrayView {
 }
 module AV = Kuiper.ArrayView
 
+(* Description of shared memory used in this kernel. *)
+inline_for_extraction noextract
+let shmems_desc (et:Type0) {| sized et |} (tile:valid_tile) : list shmem_desc = [
+  SHArray et (2sz *^ tile *^ tile);
+]
+
 (* The barrier flip-flops between an initial state
 where every threads shares all of the array, and
 a second state where each thread owns two cells
@@ -150,14 +156,14 @@ let kpre
   (eA : ematrix4 et mrows mshared tile tile)
   (eB : ematrix4 et mshared mcols tile tile)
   (fA fB : perm)
-  (ar : gpu_array et (2 * tile * tile))
+  (sh : c_shmems (shmems_desc et tile))
   (bid : natlt (mrows * mcols))
   (tid : natlt tile)
   : slprop
   =
   kpre1 comb tile gA gB gC eA eB fA fB bid tid **
-  (exists* x. gpu_pts_to_slice ar #(1.0R /. tile) 0 (2 * tile * tile) x) **
-  barrier_tok tile ar 0 tid
+  (exists* x. gpu_pts_to_slice (fst sh) #(1.0R /. tile) 0 (2 * tile * tile) x) **
+  barrier_tok tile (fst sh) 0 tid
 
 
 unfold
@@ -175,14 +181,14 @@ let kpost
   (eA : ematrix4 et mrows mshared tile tile)
   (eB : ematrix4 et mshared mcols tile tile)
   (fA fB : perm)
-  (ar : gpu_array et (2 * tile * tile))
+  (sh : c_shmems (shmems_desc et tile))
   (bid : natlt (mrows * mcols))
   (tid : natlt tile)
   : slprop
   =
   kpost1 comb tile gA gB gC eA eB fA fB bid tid **
-  (exists* x. gpu_pts_to_slice ar #(1.0R /. tile) 0 (2 * tile * tile) x) **
-  barrier_tok tile ar (2 * mshared) tid
+  (exists* x. gpu_pts_to_slice (fst sh) #(1.0R /. tile) 0 (2 * tile * tile) x) **
+  barrier_tok tile (fst sh) (2 * mshared) tid
 
 inline_for_extraction noextract
 fn eqplus
@@ -328,21 +334,24 @@ fn kf
   (gC : gpu_matrix4 et lC)
   (#eA : ematrix4 et mrows   mshared tile tile)
   (#eB : ematrix4 et mshared mcols   tile tile)
-  (ar0 : gpu_array et (2 * tile * tile))
+  (sh : c_shmems (shmems_desc et tile))
   (bid : szlt (mrows * mcols))
   (tid : szlt tile)
   ()
   requires
     gpu **
-    kpre comb tile gA gB gC eA eB fA fB ar0 bid tid **
+    kpre comb tile gA gB gC eA eB fA fB sh bid tid **
     thread_id tile tid **
     block_id (mrows * mcols) bid
   ensures
     gpu **
-    kpost comb tile gA gB gC eA eB fA fB ar0 bid tid **
+    kpost comb tile gA gB gC eA eB fA fB sh bid tid **
     thread_id tile tid **
     block_id (mrows * mcols) bid
 {
+  let ar0 : gpu_array et (2 * tile * tile) = fst sh;
+  rewrite each fst sh as ar0;
+
   gpu_pts_to_ref ar0;
 
   unfold barrier_tok tile ar0 0 tid;
@@ -465,6 +474,7 @@ fn kf
       gpu_pts_to_array ar0 #(1.0R /. tile) x1;
   fold barrier_tok tile ar0 (2 * mshared) tid;
 
+  rewrite each ar0 as (fst sh);
   ()
 }
 
@@ -519,18 +529,18 @@ fn block_setup
   (#eA : ematrix4 et mrows   mshared tile tile)
   (#eB : ematrix4 et mshared mcols   tile tile)
   (#eC : ematrix4 et mrows   mcols   tile tile)
-  (ar : gpu_array et (2 * tile * tile))
+  (sh : c_shmems (shmems_desc et tile))
   (bid : natlt (mrows * mcols))
   ()
   requires
     block_setup_tok tile **
-    (exists* v. ar |-> v) **
+    live_c_shmems sh **
     (forall+ (tid : natlt tile).
       kpre1 comb tile gA gB gC eA eB fA fB bid tid)
   ensures
     block_setup_tok tile **
     (forall+ (tid : natlt tile).
-      kpre comb tile gA gB gC eA eB fA fB ar bid tid) **
+      kpre comb tile gA gB gC eA eB fA fB sh bid tid) **
     emp (* frame *)
 {
   admit();
@@ -554,15 +564,15 @@ fn block_teardown
   (#eA : ematrix4 et mrows   mshared tile tile)
   (#eB : ematrix4 et mshared mcols   tile tile)
   (#eC : ematrix4 et mrows   mcols   tile tile)
-  (ar : gpu_array et (2 * tile * tile))
+  (sh : c_shmems (shmems_desc et tile))
   (bid : natlt (mrows * mcols))
   ()
   requires
     (forall+ (tid : natlt tile).
-      kpost comb tile gA gB gC eA eB fA fB ar bid tid) **
+      kpost comb tile gA gB gC eA eB fA fB sh bid tid) **
     emp (* frame *)
   ensures
-    (exists* v. gpu_pts_to_array ar #1.0R v) **
+    live_c_shmems sh **
     (forall+ (tid : natlt tile).
       kpost1 comb tile gA gB gC eA eB fA fB bid tid)
 {
@@ -635,9 +645,7 @@ let mk_kernel
   nblk = mrows *^ mcols;
   nthr = tile;
 
-  shmem_type = et;
-  shmem_type_is_sized = solve;
-  shmem_sz = (2sz *^ tile *^ tile);
+  shmems_desc = shmems_desc et tile;
 
   frame = emp;
   block_pre  = (fun bid -> forall+ (tid : natlt tile). kpre1  comb tile gA gB gC eA eB fA fB bid tid);
